src/single_auth_message/DY.Example.SingleAuthMessage.SecurityProperties.fst
@@ -8,18 +8,42 @@ open DY.Example.SingleAuthMessage.Protocol.Total.Proof
 open DY.Example.SingleAuthMessage.Protocol.Stateful
 open DY.Example.SingleAuthMessage.Protocol.Stateful.Proof
 
-#set-options "--fuel 0 --ifuel 0 --z3rlimit 10  --z3cliopt 'smt.qi.eager_threshold=100'"
+#set-options "--fuel 0 --ifuel 0 --z3rlimit 10 --z3cliopt 'smt.qi.eager_threshold=100'"
 
+// For authenticated messages we can prove on the
+// receiver side that either the sender triggered
+// a send event or the sender is corrupt.
 val sender_authentication:
-  tr:trace -> sender:principal -> receiver:principal -> secret:bytes ->
+  tr:trace -> i:timestamp ->
+  sender:principal -> receiver:principal ->
+  secret:bytes ->
   Lemma
   (requires
     trace_invariant tr /\
-    event_triggered tr receiver (ReceiverReceivedMsg sender receiver secret (compute_message secret))
+    event_triggered_at tr i receiver (ReceiverReceivedMsg sender receiver secret (compute_message secret))
   )
   (ensures
     event_triggered tr sender (SenderSendMsg sender secret) \/
-    (exists vk_sender. event_triggered tr receiver (CommAuthReceiveMsg sender receiver vk_sender (compute_message secret)) /\
-      is_corrupt tr (get_signkey_label vk_sender))
+    is_corrupt tr (principal_label sender)
   )
-let sender_authentication tr sender receiver secret = ()
+let sender_authentication tr i sender receiver secret = ()
+
+// This is the same securtiy lemma as above but
+// with the events from the communication layer.
+// This allows us to argue with the `(prefix tr i)`
+// function. (Not sure why this does not work
+// in the lemma above)
+val sender_authentication':
+  tr:trace -> i:timestamp ->
+  sender:principal -> receiver:principal ->
+  payload:bytes ->
+  Lemma
+  (requires
+    trace_invariant tr /\
+    event_triggered_at tr i receiver (CommAuthReceiveMsg sender receiver payload)
+  )
+  (ensures
+    event_triggered (prefix tr i) sender (CommAuthSendMsg sender payload) \/
+    is_corrupt (prefix tr i) (principal_label sender)
+  )
+let sender_authentication' tr i sender receiver payload = ()
