src/single_conf_message/DY.Example.SingleConfMessage.SecurityProperties.fst
@@ -10,21 +10,18 @@ open DY.Example.SingleConfMessage.Protocol.Stateful.Proof
 
 #set-options "--fuel 0 --ifuel 0 --z3rlimit 10  --z3cliopt 'smt.qi.eager_threshold=100'"
 
-val receiver_authentication:
-  tr:trace ->
-  sender:principal -> receiver:principal ->
-  secret:bytes ->
-  Lemma
-  (requires
-    trace_invariant tr /\
-    event_triggered tr receiver (ReceiverReceivedMsg sender receiver secret (compute_message secret))
-  )
-  (ensures
-    event_triggered tr sender (SenderSendMsg sender receiver secret) \/
-    is_publishable tr (compute_message secret)
-  )
-let receiver_authentication tr sender receiver secret = ()
-
+// This is the main security property of a
+// confidential message. It states from the sender
+// perspective that the secret is not leaked to
+// the attacker as long as the sender and receiver
+// are honest.
+//
+// **Note:** We know that if the receiver is
+// honest only the receiver can decrypt the
+// secret. This allows us to argue from the
+// sender's perspective that if the attacker knows
+// the secret either the sender or the receiver is
+// corrupt.
 val secret_secrecy_sender:
   tr:trace -> sender:principal -> receiver:principal -> secret:bytes ->
   Lemma
@@ -39,3 +36,72 @@ val secret_secrecy_sender:
 let secret_secrecy_sender tr sender receiver secret =
   attacker_only_knows_publishable_values tr secret;
   ()
+
+// On the receiver side we don't have any
+// guarantees on the secrecy of the secret. We can
+// only prove that if the attacker knows the
+// secret, it is publishable.
+val secret_secrecy_receiver:
+  tr:trace -> sender:principal -> receiver:principal -> secret:bytes ->
+  Lemma
+  (requires
+    trace_invariant tr /\
+    attacker_knows tr secret
+  )
+  (ensures
+    is_publishable tr secret
+  )
+let secret_secrecy_receiver tr sender receiver secret =
+  attacker_only_knows_publishable_values tr secret;
+  ()
+
+// We can also not authenticate the sender because
+// the attacker could write an arbitrary sender in
+// the message. The only thing we can prove is
+// that if the secret is not publisable, the
+// sender contained in the message triggered an
+// event.
+val sender_authentication:
+  tr:trace ->
+  sender:principal -> receiver:principal ->
+  secret:bytes ->
+  Lemma
+  (requires
+    trace_invariant tr /\
+    event_triggered tr receiver (ReceiverReceivedMsg sender receiver secret (compute_message secret))
+  )
+  (ensures
+    event_triggered tr sender (SenderSendMsg sender receiver secret) \/
+    is_publishable tr (compute_message secret)
+    // We cannot prove `is_corrupt tr
+    // (principal_label sender)` because the
+    // sender is not authenticated. If the
+    // attacker creates this message, they can
+    // choose an arbitrary sender for the sender
+    // field.
+  )
+let sender_authentication tr sender receiver secret = ()
+
+(*
+
+// This is not provable because the receiver event
+// is in the future, and it is not guaranteed that
+// it is ever triggered.
+
+val recever_authentication:
+  tr:trace ->
+  sender:principal -> receiver:principal ->
+  secret:bytes ->
+  Lemma
+  (requires
+    trace_invariant tr /\
+    event_triggered tr sender (SenderSendMsg sender receiver secret)
+    
+  )
+  (ensures
+    event_triggered tr receiver (ReceiverReceivedMsg sender receiver secret (compute_message secret)) \/
+    is_corrupt tr (principal_label receiver)
+    //is_publishable tr (compute_message secret)
+  )
+let recever_authentication tr sender receiver secret = ()
+*)
