README.md
@@ -1,0 +1,13 @@
+# DY* Communication Layer Examples
+
+This repository contains examples that show
+how the DY* communication layer can be used.
+Currently, the following examples are
+implemented:
+
+- Minimal example for the
+  [confidential](src/single_conf_message/)
+  send and receive functions
+- Minimal example for the
+  [authenticated](src/single_auth_message/)
+  send and receive functions
